Switch to metalib library from TLC

Definitions.v
@@ -2,9 +2,7 @@ From Coq Require Import List.
 Import ListNotations.
 Import Nat.
 
-From TLC Require Export LibFix.
-From TLC Require Export LibVar.
-From TLC Require Export LibFset.
+From Metalib Require Export Metatheory.
 
 (*
 Defines the syntax of our source and target languages,
@@ -23,7 +21,7 @@ Cofinite Quantification
   which gives us a stronger induction hypothesis
 *)
 
-Implicit Types x y z : var.
+(* Implicit Types x y z : var. *)
 
 (*
 pre terms may contain non locally closed terms
@@ -60,33 +58,6 @@ Inductive s_trm : Set :=
 Notation "` ( t ) " := (s_trm_seq [t]).
 Notation "` ( t1 ; t2 ; .. ; t3 )" := (s_trm_seq (cons t1 (cons t2 .. (cons t3 nil) ..))).
 
-(* target language pre-terms
-   add let, set! is now only on free vars, so call it set_top *)
-Inductive t_trm : Set :=
-  (* non-values *)
-  | t_trm_seq (ts : list t_trm)
-  | t_trm_begin (ts : list t_trm)
-  | t_trm_set_top (x : t_trm) (t : t_trm)
-  | t_trm_var (x : ln_var)
-  | t_trm_let (v : t_trm) (ts : list t_trm)
-
-  (* values *)
-  | t_trm_abs  (ts : list t_trm)
-  | t_trm_setcar
-  | t_trm_setcdr
-  | t_trm_cons
-  | t_trm_car 
-  | t_trm_cdr 
-  | t_trm_pp (n : var)
-  | t_trm_num (i : nat)
-  | t_trm_null
-  | t_trm_true
-  | t_trm_false.
-
-Notation "$ { t } " := (t_trm_seq [t]).
-Notation "$ { t1 ; t2 ; .. ; t3 }" := (t_trm_seq (cons t1 (cons t2 .. (cons t3 nil) ..))).
-  
-
 (* values in source language *)
 Inductive value : s_trm -> Prop :=
   | val_abs : forall ts,
@@ -111,18 +82,6 @@ with vals : list s_trm -> Prop :=
         value t ->
         vals (t :: ts).
 
-(*
-Inductive t_val : t_trm -> Prop :=
-  | tval_abs : forall ts,
-      t_val (t_trm_abs ts)
-  | tval_pp : forall n,
-      t_val (t_trm_pp n)
-  | tval_num : forall i,
-      t_val (t_trm_num i)
-  | tval_null : t_val (t_trm_null)
-  | tval_true : t_val (t_trm_true)
-  | tval_false : t_val (t_trm_false).
-*)
 
 (* 
 Opening a trm t with a trm u containing a fresh free variable x.
@@ -141,12 +100,12 @@ Definition open_var v k (u t : s_trm) :=
 Fixpoint s_open_rec (k : nat) (u : s_trm) (t : s_trm) {struct t} : s_trm :=
   match t with
   (* for lists of terms that don't abstract, just apply open to all terms *)
-  | s_trm_seq ts => s_trm_seq (map (s_open_rec k u) ts)
-  | s_trm_begin ts => s_trm_begin (map (s_open_rec k u) ts)
+  | s_trm_seq ts => s_trm_seq (List.map (s_open_rec k u) ts)
+  | s_trm_begin ts => s_trm_begin (List.map (s_open_rec k u) ts)
 
   (* since lambda abstracts, add a layer of depth *)
   | s_trm_abs ts => let s_open_rec_S := (s_open_rec (S k) u) in
-                    s_trm_abs (map s_open_rec_S ts)
+                    s_trm_abs (List.map s_open_rec_S ts)
   
   (* for set!, just apply open to args*)
   | s_trm_set x t1 => s_trm_set (s_open_rec k u x) (s_open_rec k u t1)
@@ -162,6 +121,12 @@ Fixpoint s_open_rec (k : nat) (u : s_trm) (t : s_trm) {struct t} : s_trm :=
 
 (* open a term t with another term u at base level of abstraction *)
 Definition open t u := s_open_rec 0 u t.
+
+Fixpoint open_each ts u :=
+  match ts with
+  | [] => []
+  | t :: ts' => (open t u) :: (open_each ts' u)
+  end.
 
 (* open a term t with some fvar x *)
 Notation "t ^^ x" := (open t (s_trm_var (fvar x))) (at level 67).
@@ -180,19 +145,19 @@ Replaces a free var z with bvar k where k is the current level of abstraction
 Fixpoint s_close_var_rec (k : nat) (z : var) (t : s_trm) {struct t} : s_trm :=
   match t with
   (* seq and begin don't abstract, so just call on each term *)
-  | s_trm_seq ts => s_trm_seq (map (s_close_var_rec k z) ts)
-  | s_trm_begin ts => s_trm_begin (map (s_close_var_rec k z) ts)
+  | s_trm_seq ts => s_trm_seq (List.map (s_close_var_rec k z) ts)
+  | s_trm_begin ts => s_trm_begin (List.map (s_close_var_rec k z) ts)
 
   (* lambda abstracts, so increment depth and then call on each term *)
   | s_trm_abs ts => let s_close_var_rec_S := (s_close_var_rec (S k) z) in
-                    s_trm_abs (map s_close_var_rec_S ts)
+                    s_trm_abs (List.map s_close_var_rec_S ts)
 
   (* apply close to set's variable and body *)
   | s_trm_set x t1 => s_trm_set (s_close_var_rec k z x) (s_close_var_rec k z t1)
 
   (* replace fvar z with bvar k *)
   | s_trm_var v => match v with
-                   | fvar x => if var_compare x z then (s_trm_var (bvar k)) else t
+                   | fvar x => if (x == z) then (s_trm_var (bvar k)) else t
                    | bvar _ => t
                    end
   | _ => t
@@ -259,25 +224,25 @@ Definition s_body ts :=
 Fixpoint s_fv (t : s_trm) : vars :=
   let fix fvs' (ts : list s_trm) : vars :=
     match ts with
-    | [] => \{}
+    | [] => {}
     | t :: ts' => s_fv t \u fvs' ts'
     end
   in
     match t with
     | s_trm_var v => match v with
-                     | fvar y => \{y}
-                     | bvar _ => \{}
+                     | fvar y => {{ y }}
+                     | bvar _ => {}
                      end
     | s_trm_abs ts => fvs' ts
     | s_trm_begin ts => fvs' ts
     | s_trm_seq ts => fvs' ts
     | s_trm_set x t1 => (s_fv x) \u (s_fv t1)
-    | _ => \{}
+    | _ => {}
     end.
 
 Fixpoint s_fvs ts :=
   match ts with
-  | [] => \{}
+  | [] => {}
   | t :: ts' => s_fv t \u s_fvs ts'
   end.
 
@@ -290,7 +255,7 @@ Fixpoint s_subst (z : var) (u : s_trm) (t : s_trm) {struct t} : s_trm :=
   in
   match t with
   | s_trm_var v => match v with
-                   | fvar x => if (var_compare x z) then u else t
+                   | fvar x => if (x == z) then u else t
                    | bvar _ => t
                    end
   | s_trm_abs ts => s_trm_abs (substs ts)
@@ -313,184 +278,9 @@ Definition sum (l : list nat) :=
 
 Fixpoint s_trm_size (t : s_trm) {struct t} : nat :=
   match t with
-  | s_trm_abs ts => 1 + (sum (map s_trm_size ts))
-  | s_trm_begin ts => 1 + (sum (map s_trm_size ts))
-  | s_trm_seq ts => 1 + (sum (map s_trm_size ts))
+  | s_trm_abs ts => 1 + (sum (List.map s_trm_size ts))
+  | s_trm_begin ts => 1 + (sum (List.map s_trm_size ts))
+  | s_trm_seq ts => 1 + (sum (List.map s_trm_size ts))
   | s_trm_set x t1 => 1 + (s_trm_size x) + (s_trm_size t1)
   | _ => 1
   end.
-
-
-
-(* probably not needed target language stuff 
-
-Fixpoint t_open_rec (k : nat) (u : t_trm) (t : t_trm) {struct t} : t_trm :=
-  match t with
-  | t_trm_bvar i => if (k =? i) then u else t
-  | t_trm_fvar x => t
-  | t_trm_abs ts => let t_open_rec_S := (t_open_rec (S k) u) in
-                    t_trm_abs (map t_open_rec_S ts)
-  | t_trm_let v ts => let t_open_rec_S := (t_open_rec (S k) u) in
-                      t_trm_let (t_open_rec k u v) (map t_open_rec_S ts)
-  | t_trm_set_top x t1 => t_trm_set_top x (t_open_rec k u t1)
-  | t_trm_app t1 t2 => t_trm_app (t_open_rec k u t1)(t_open_rec k u t2)
-  | t_trm_setcar p v => t_trm_setcar (t_open_rec k u p) (t_open_rec k u v)
-  | t_trm_setcdr p v => t_trm_setcdr (t_open_rec k u p) (t_open_rec k u v)
-  | t_trm_cons v1 v2 => t_trm_cons (t_open_rec k u v1)(t_open_rec k u v2)
-  | t_trm_car p => t_trm_car (t_open_rec k u p)
-  | t_trm_cdr p => t_trm_cdr (t_open_rec k u p)
-  | t_trm_begin ts => let t_open_rec_S := (t_open_rec (S k) u) in
-                      t_trm_begin (map t_open_rec_S ts)
-  | _ => t
-  end.
-
-Notation "{ k ~>t u } t" := (t_open_rec k u t) (at level 67).
-
-Definition t_open t u := t_open_rec 0 u t.
-
-Notation "t ^^t u" := (t_open t u) (at level 67).
-Notation "t ^t x" := (t_open t (t_trm_fvar x)) (at level 67).
-
-
-Fixpoint t_close_var_rec (k : nat) (z : var) (t : t_trm) {struct t} : t_trm :=
-  match t with
-  | t_trm_bvar i => t
-  | t_trm_fvar x => if var_compare x z then (t_trm_bvar k) else t
-  | t_trm_abs ts => let t_close_var_rec_S := (t_close_var_rec (S k) z) in
-                  t_trm_abs (map t_close_var_rec_S ts)
-  | t_trm_app t1 t2 => t_trm_app (t_close_var_rec k z t1) (t_close_var_rec k z t2)
-  | t_trm_setcar p v => t_trm_setcar (t_close_var_rec k z p) (t_close_var_rec k z v)
-  | t_trm_setcdr p v => t_trm_setcdr (t_close_var_rec k z p) (t_close_var_rec k z v)
-  | t_trm_cons v1 v2 => t_trm_cons (t_close_var_rec k z v1) (t_close_var_rec k z v2)
-  | t_trm_car p => t_trm_car (t_close_var_rec k z p)
-  | t_trm_cdr p => t_trm_cdr (t_close_var_rec k z p)
-  | t_trm_begin ts => t_trm_begin (map (t_close_var_rec k z) ts)
-  | _ => t
-  end.
-
-
-Definition t_close_var z t := t_close_var_rec 0 z t.
-
-Fixpoint t_open_each ts x :=
-  match ts with
-  | [] => []
-  | t :: ts' => (t ^t x) :: t_open_each ts' x
-  end.
-
-Fixpoint t_open_each_term ts u :=
-  match ts with
-  | [] => []
-  | t :: ts' => (t ^^s u) :: t_open_each_term ts' u
-  end.
-
-Inductive t_term : t_trm -> Prop :=
-  | t_term_fvar : forall x,
-      t_term (t_trm_fvar x)
-  | t_term_app : forall t1 t2,
-      t_term t1 -> t_term t2 -> t_term (t_trm_app t1 t2)
-  | t_term_abs : forall L ts,
-      (forall x, x \notin L -> t_terms (t_open_each ts x)) ->
-      t_term (t_trm_abs ts)
-  | t_term_begin : forall L ts,
-      (forall x, x \notin L -> t_terms (t_open_each ts x)) ->
-      t_term (t_trm_begin ts)
-  | t_term_let : forall L ts t b,
-      t_term b ->
-      In t ts ->
-      (forall x, x \notin L -> t_terms (t_open_each ts x)) ->
-      t_term (t_trm_let b ts)
-  | t_term_setcar : forall p v,
-      t_term p -> t_term v -> t_term (t_trm_setcar p v)
-  | t_term_setcdr : forall p v,
-      t_term p -> t_term v -> t_term (t_trm_setcdr p v)
-  | t_term_cons : forall v1 v2, 
-      t_term v1 -> t_term v2 -> t_term (t_trm_cons v1 v2)
-  | t_term_car : forall p,
-      t_term p -> t_term (t_trm_car p)
-  | t_term_cdr : forall p,
-      t_term p -> t_term (t_trm_cdr p)
-  | t_term_pp : forall n,
-      t_term (t_trm_pp n)
-  | t_term_num : forall i,
-      t_term (t_trm_num i)
-  | t_term_null : t_term (t_trm_null)
-  | t_term_true : t_term (t_trm_true)
-  | t_term_false : t_term (t_trm_false)
-
-with t_terms : list t_trm -> Prop :=
-  | t_terms_nil : t_terms ([])
-  | t_terms_single : forall t, t_term t -> t_terms [t]
-  | t_terms_next : 
-      forall t ts,
-        t_terms ts -> 
-        t_term t ->
-        t_terms (t :: ts).
-
-Definition t_body ts :=
-  exists L,
-  forall x, x \notin L -> t_terms (t_open_each ts x).
-
-Fixpoint t_fv (t : t_trm) : vars :=
-  let fix fvs' (ts : list t_trm) : vars :=
-    match ts with
-    | [] => \{}
-    | t :: ts' => t_fv t \u fvs' ts'
-    end
-  in
-    match t with
-    | t_trm_fvar y => \{y}
-    | t_trm_bvar _ => \{}
-    | t_trm_abs ts => fvs' ts
-    | t_trm_begin ts => fvs' ts
-    | t_trm_app t1 t2 => (t_fv t1) \u (t_fv t2)
-    | t_trm_set_top x t1 => \{x} \u (t_fv t1)
-    | t_trm_setcar p v => (t_fv p) \u (t_fv v)
-    | t_trm_setcdr p v => (t_fv p) \u (t_fv v)
-    | t_trm_cons v1 v2 => (t_fv v1) \u (t_fv v2)
-    | t_trm_car p => t_fv p
-    | t_trm_cdr p => t_fv p
-    | _ => \{}
-    end.
-
-Fixpoint t_subst (z : var) (u : t_trm) (t : t_trm) {struct t} : t_trm :=
-  let fix substs (ts : list t_trm) :=
-    match ts with
-    | [] => []
-    | t' :: ts' => (t_subst z u t') :: (substs ts')
-    end
-  in
-  match t with
-  | t_trm_abs ts => t_trm_abs (substs ts)
-  | t_trm_begin ts => t_trm_begin (substs ts)
-  | t_trm_app t1 t2 => t_trm_app (t_subst z u t1) (t_subst z u t2)
-  | t_trm_let v ts => t_trm_let (t_subst z u v) (substs ts)
-  | t_trm_setcar p v => t_trm_setcar (t_subst z u p) (t_subst z u v)
-  | t_trm_setcdr p v => t_trm_setcdr (t_subst z u p) (t_subst z u v)
-  | t_trm_cons v1 v2 => t_trm_cons (t_subst z u v1) (t_subst z u v2)
-  | t_trm_car p => t_trm_car (t_subst z u p)
-  | t_trm_cdr p => t_trm_cdr (t_subst z u p)
-  | t_trm_fvar x => if (var_compare x z) then u else t
-  | t_trm_bvar i => t
-  | _ => t
-  end.
-
-Notation "[ z ~>t u ] t" := (t_subst z u t) (at level 68).
-
-Fixpoint t_trm_size (t : t_trm) {struct t} : nat :=
-  match t with 
-  | t_trm_abs ts => 1 + (sum (map t_trm_size ts))
-  | t_trm_begin ts => 1 + (sum (map t_trm_size ts))
-  | t_trm_app t1 t2 => 1 + (t_trm_size t1) + (t_trm_size t2)
-  | t_trm_set_top x t1 => 2 + (t_trm_size t1)
-  | t_trm_let v ts => 1 + (t_trm_size v) + (sum (map t_trm_size ts))
-  | t_trm_setcar p v => 1 + (t_trm_size p) + (t_trm_size v)
-  | t_trm_setcdr p v => 1 + (t_trm_size p) + (t_trm_size v)
-  | t_trm_cons v1 v2 => 1 + (t_trm_size v1) + (t_trm_size v2)
-  | t_trm_car p => 1 + (t_trm_size p)
-  | t_trm_cdr p => 1 + (t_trm_size p)
-  | t_trm_fvar _ => 1
-  | t_trm_bvar _ => 1
-  | _ => 1
-  end.
-
-*)
