Pass.v
@@ -24,7 +24,7 @@ Fixpoint has_assigning_set (n i : nat) (t : s_trm) :=
     | s_trm_begin ts => has_assigning_set_list n' i ts
     | s_trm_abs ts => has_assigning_set_list n' (S i) ts
     | s_trm_set x t1 => match x with
-                      | (s_trm_var (bvar n)) => if (i =? n) then SomeE true else has_assigning_set n' i t1
+                      | (s_trm_var (bvar n)) => if (i == n) then SomeE true else has_assigning_set n' i t1
                       | _ => has_assigning_set n' i t1
                       end
     | _ => SomeE false
@@ -64,14 +64,14 @@ Fixpoint handle_assigning_set (n i : nat) (t : s_trm) :=
     | s_trm_set x t1 => ' t1' <- (handle_assigning_set n' i t1) ;;
                         match x with
                         | (s_trm_var (bvar a)) => 
-                            if (a =? i)
+                            if (a == i)
                             then SomeE ` (s_trm_setcar ; x ; t1') 
                             else SomeE (s_trm_set x t1')
                         | _ => SomeE (s_trm_set x t1')
                         end
           
     | s_trm_var v => match v with
-                     | bvar a => if (a =? i)
+                     | bvar a => if (a == i)
                                  then SomeE ` (s_trm_car ; (s_trm_var (bvar a)))
                                  else SomeE t
                      | fvar _ => SomeE t
@@ -97,6 +97,34 @@ Definition handle_sets := handle_assigning_set big_num 0.
 Definition handle_sets_list := handle_assigning_set_list big_num 0.
 Definition has_sets := has_assigning_set big_num 0.
 Definition has_sets_list := has_assigning_set_list big_num 0.
+
+(* target language terms
+   add let, set! is now only on free vars, so call it set_top *)
+   Inductive t_trm : Set :=
+   (* non-values *)
+   | t_trm_seq (ts : list t_trm)
+   | t_trm_begin (ts : list t_trm)
+   | t_trm_set_top (x : t_trm) (t : t_trm)
+   | t_trm_var (x : ln_var)
+   | t_trm_let (v : t_trm) (ts : list t_trm)
+ 
+   (* values *)
+   | t_trm_abs  (ts : list t_trm)
+   | t_trm_setcar
+   | t_trm_setcdr
+   | t_trm_cons
+   | t_trm_car 
+   | t_trm_cdr 
+   | t_trm_pp (n : var)
+   | t_trm_num (i : nat)
+   | t_trm_null
+   | t_trm_true
+   | t_trm_false.
+ 
+ Notation "$ { t } " := (t_trm_seq [t]).
+ Notation "$ { t1 ; t2 ; .. ; t3 }" := (t_trm_seq (cons t1 (cons t2 .. (cons t3 nil) ..))).
+   
+ 
 
 
 (* 
@@ -219,3 +247,188 @@ Definition ca t :=
 
 Definition desugar t :=
   de_sugar big_num t.
+
+
+
+(*
+Inductive t_val : t_trm -> Prop :=
+  | tval_abs : forall ts,
+      t_val (t_trm_abs ts)
+  | tval_pp : forall n,
+      t_val (t_trm_pp n)
+  | tval_num : forall i,
+      t_val (t_trm_num i)
+  | tval_null : t_val (t_trm_null)
+  | tval_true : t_val (t_trm_true)
+  | tval_false : t_val (t_trm_false).
+
+Fixpoint t_open_rec (k : nat) (u : t_trm) (t : t_trm) {struct t} : t_trm :=
+  match t with
+  | t_trm_bvar i => if (k =? i) then u else t
+  | t_trm_fvar x => t
+  | t_trm_abs ts => let t_open_rec_S := (t_open_rec (S k) u) in
+                    t_trm_abs (map t_open_rec_S ts)
+  | t_trm_let v ts => let t_open_rec_S := (t_open_rec (S k) u) in
+                      t_trm_let (t_open_rec k u v) (map t_open_rec_S ts)
+  | t_trm_set_top x t1 => t_trm_set_top x (t_open_rec k u t1)
+  | t_trm_app t1 t2 => t_trm_app (t_open_rec k u t1)(t_open_rec k u t2)
+  | t_trm_setcar p v => t_trm_setcar (t_open_rec k u p) (t_open_rec k u v)
+  | t_trm_setcdr p v => t_trm_setcdr (t_open_rec k u p) (t_open_rec k u v)
+  | t_trm_cons v1 v2 => t_trm_cons (t_open_rec k u v1)(t_open_rec k u v2)
+  | t_trm_car p => t_trm_car (t_open_rec k u p)
+  | t_trm_cdr p => t_trm_cdr (t_open_rec k u p)
+  | t_trm_begin ts => let t_open_rec_S := (t_open_rec (S k) u) in
+                      t_trm_begin (map t_open_rec_S ts)
+  | _ => t
+  end.
+
+Notation "{ k ~>t u } t" := (t_open_rec k u t) (at level 67).
+
+Definition t_open t u := t_open_rec 0 u t.
+
+Notation "t ^^t u" := (t_open t u) (at level 67).
+Notation "t ^t x" := (t_open t (t_trm_fvar x)) (at level 67).
+
+
+Fixpoint t_close_var_rec (k : nat) (z : var) (t : t_trm) {struct t} : t_trm :=
+  match t with
+  | t_trm_bvar i => t
+  | t_trm_fvar x => if var_compare x z then (t_trm_bvar k) else t
+  | t_trm_abs ts => let t_close_var_rec_S := (t_close_var_rec (S k) z) in
+                  t_trm_abs (map t_close_var_rec_S ts)
+  | t_trm_app t1 t2 => t_trm_app (t_close_var_rec k z t1) (t_close_var_rec k z t2)
+  | t_trm_setcar p v => t_trm_setcar (t_close_var_rec k z p) (t_close_var_rec k z v)
+  | t_trm_setcdr p v => t_trm_setcdr (t_close_var_rec k z p) (t_close_var_rec k z v)
+  | t_trm_cons v1 v2 => t_trm_cons (t_close_var_rec k z v1) (t_close_var_rec k z v2)
+  | t_trm_car p => t_trm_car (t_close_var_rec k z p)
+  | t_trm_cdr p => t_trm_cdr (t_close_var_rec k z p)
+  | t_trm_begin ts => t_trm_begin (map (t_close_var_rec k z) ts)
+  | _ => t
+  end.
+
+
+Definition t_close_var z t := t_close_var_rec 0 z t.
+
+Fixpoint t_open_each ts x :=
+  match ts with
+  | [] => []
+  | t :: ts' => (t ^t x) :: t_open_each ts' x
+  end.
+
+Fixpoint t_open_each_term ts u :=
+  match ts with
+  | [] => []
+  | t :: ts' => (t ^^s u) :: t_open_each_term ts' u
+  end.
+
+Inductive t_term : t_trm -> Prop :=
+  | t_term_fvar : forall x,
+      t_term (t_trm_fvar x)
+  | t_term_app : forall t1 t2,
+      t_term t1 -> t_term t2 -> t_term (t_trm_app t1 t2)
+  | t_term_abs : forall L ts,
+      (forall x, x \notin L -> t_terms (t_open_each ts x)) ->
+      t_term (t_trm_abs ts)
+  | t_term_begin : forall L ts,
+      (forall x, x \notin L -> t_terms (t_open_each ts x)) ->
+      t_term (t_trm_begin ts)
+  | t_term_let : forall L ts t b,
+      t_term b ->
+      In t ts ->
+      (forall x, x \notin L -> t_terms (t_open_each ts x)) ->
+      t_term (t_trm_let b ts)
+  | t_term_setcar : forall p v,
+      t_term p -> t_term v -> t_term (t_trm_setcar p v)
+  | t_term_setcdr : forall p v,
+      t_term p -> t_term v -> t_term (t_trm_setcdr p v)
+  | t_term_cons : forall v1 v2, 
+      t_term v1 -> t_term v2 -> t_term (t_trm_cons v1 v2)
+  | t_term_car : forall p,
+      t_term p -> t_term (t_trm_car p)
+  | t_term_cdr : forall p,
+      t_term p -> t_term (t_trm_cdr p)
+  | t_term_pp : forall n,
+      t_term (t_trm_pp n)
+  | t_term_num : forall i,
+      t_term (t_trm_num i)
+  | t_term_null : t_term (t_trm_null)
+  | t_term_true : t_term (t_trm_true)
+  | t_term_false : t_term (t_trm_false)
+
+with t_terms : list t_trm -> Prop :=
+  | t_terms_nil : t_terms ([])
+  | t_terms_single : forall t, t_term t -> t_terms [t]
+  | t_terms_next : 
+      forall t ts,
+        t_terms ts -> 
+        t_term t ->
+        t_terms (t :: ts).
+
+Definition t_body ts :=
+  exists L,
+  forall x, x \notin L -> t_terms (t_open_each ts x).
+
+Fixpoint t_fv (t : t_trm) : vars :=
+  let fix fvs' (ts : list t_trm) : vars :=
+    match ts with
+    | [] => \{}
+    | t :: ts' => t_fv t \u fvs' ts'
+    end
+  in
+    match t with
+    | t_trm_fvar y => \{y}
+    | t_trm_bvar _ => \{}
+    | t_trm_abs ts => fvs' ts
+    | t_trm_begin ts => fvs' ts
+    | t_trm_app t1 t2 => (t_fv t1) \u (t_fv t2)
+    | t_trm_set_top x t1 => \{x} \u (t_fv t1)
+    | t_trm_setcar p v => (t_fv p) \u (t_fv v)
+    | t_trm_setcdr p v => (t_fv p) \u (t_fv v)
+    | t_trm_cons v1 v2 => (t_fv v1) \u (t_fv v2)
+    | t_trm_car p => t_fv p
+    | t_trm_cdr p => t_fv p
+    | _ => \{}
+    end.
+
+Fixpoint t_subst (z : var) (u : t_trm) (t : t_trm) {struct t} : t_trm :=
+  let fix substs (ts : list t_trm) :=
+    match ts with
+    | [] => []
+    | t' :: ts' => (t_subst z u t') :: (substs ts')
+    end
+  in
+  match t with
+  | t_trm_abs ts => t_trm_abs (substs ts)
+  | t_trm_begin ts => t_trm_begin (substs ts)
+  | t_trm_app t1 t2 => t_trm_app (t_subst z u t1) (t_subst z u t2)
+  | t_trm_let v ts => t_trm_let (t_subst z u v) (substs ts)
+  | t_trm_setcar p v => t_trm_setcar (t_subst z u p) (t_subst z u v)
+  | t_trm_setcdr p v => t_trm_setcdr (t_subst z u p) (t_subst z u v)
+  | t_trm_cons v1 v2 => t_trm_cons (t_subst z u v1) (t_subst z u v2)
+  | t_trm_car p => t_trm_car (t_subst z u p)
+  | t_trm_cdr p => t_trm_cdr (t_subst z u p)
+  | t_trm_fvar x => if (var_compare x z) then u else t
+  | t_trm_bvar i => t
+  | _ => t
+  end.
+
+Notation "[ z ~>t u ] t" := (t_subst z u t) (at level 68).
+
+Fixpoint t_trm_size (t : t_trm) {struct t} : nat :=
+  match t with 
+  | t_trm_abs ts => 1 + (sum (map t_trm_size ts))
+  | t_trm_begin ts => 1 + (sum (map t_trm_size ts))
+  | t_trm_app t1 t2 => 1 + (t_trm_size t1) + (t_trm_size t2)
+  | t_trm_set_top x t1 => 2 + (t_trm_size t1)
+  | t_trm_let v ts => 1 + (t_trm_size v) + (sum (map t_trm_size ts))
+  | t_trm_setcar p v => 1 + (t_trm_size p) + (t_trm_size v)
+  | t_trm_setcdr p v => 1 + (t_trm_size p) + (t_trm_size v)
+  | t_trm_cons v1 v2 => 1 + (t_trm_size v1) + (t_trm_size v2)
+  | t_trm_car p => 1 + (t_trm_size p)
+  | t_trm_cdr p => 1 + (t_trm_size p)
+  | t_trm_fvar _ => 1
+  | t_trm_bvar _ => 1
+  | _ => 1
+  end.
+
+*)
